remove ops

CryptoPrims/AuthEnc.lean
@@ -1,29 +1,5 @@
 import OwlLean.TypeChecker.OwlComplete
 
-def genKey : Owl.op :=
-  fun (_ _ : Owl.binary) =>
-    Owl.Dist.ret (Owl.binary.bend)
-
--- non functional
-def enc : Owl.op :=
-  fun (_ _ : Owl.binary) =>
-    Owl.Dist.ret (Owl.binary.bend)
-
--- non functional
-def dec : Owl.op :=
-  fun (_ _ : Owl.binary) =>
-    Owl.Dist.ret (Owl.binary.bend)
-
--- non functional
-def rand : Owl.op :=
-  fun (_ _ : Owl.binary) =>
-    Owl.Dist.ret (Owl.binary.bend)
-
--- non functional
-def eq : Owl.op :=
-  fun (_ _ : Owl.binary) =>
-    Owl.Dist.ret (Owl.binary.bend)
-
 def ENC :=
   OwlTy [lK, lM] [tau] {
     (∃ alphaK <: (Data lK) .
@@ -34,21 +10,21 @@ def ENC :=
 
 def EncIdeal :=
   Owl [lK, lM] [tau] [] {
-    let k = (⟨genKey⟩ (["0"], ["0"]) : Data lK) in
+    let k = (⟨"genKey"⟩ (["0"], ["0"]) : Data lK) in
     let L = alloc (λ (null : Public) : (tau + Unit) => ı2 *) in
     let enc' = (if corr (lK) then
-                  (λ (x : Public * Public) : Public => ⟨enc⟩ (π1 x, π2 x))
+                  (λ (x : Public * Public) : Public => ⟨"enc"⟩ (π1 x, π2 x))
                 else
                   λ (x : (Data lK * tau)) : Public =>
-                    let c = ⟨rand⟩ (zero ((π2 x) : Data lM), ["0"]) in
+                    let c = ⟨"rand"⟩ (zero ((π2 x) : Data lM), ["0"]) in
                     let L_old = (! L) in
                     let u = L := (λ (y : Public) : (tau + Unit) =>
-                        if ⟨eq⟩(y, c) then ı1 (π2 x) else L_old [y])
+                        if ⟨"eq"⟩(y, c) then ı1 (π2 x) else L_old [y])
                     in
                     c)
     in
     let dec' = (if corr (lK) then
-                  λ (x : Public * Public) : Public => ⟨dec⟩ (π1 x, π2 x)
+                  λ (x : Public * Public) : Public => ⟨"dec"⟩ (π1 x, π2 x)
                 else
                   λ (x : (Data lK * Public)) : (tau + Unit) => (!L) [π2 x])
     in
